Progress on stateful incremental Blake2s

code/hash/Hacl.Blake2s.fst
@@ -3,23 +3,24 @@ module Hacl.Blake2s
 open FStar.Mul
 open FStar.HyperStack
 open FStar.HyperStack.ST
+
 open Spec.Lib.IntTypes
-open Spec.Lib.IntSeq
-
 open Spec.Lib.IntBuf
-open Spec.Lib.IntBuf.Lemmas
-open Spec.Lib.IntBuf.LoadStore
 
-module ST = FStar.HyperStack.ST
-module LSeq = Spec.Lib.IntSeq
 module Spec = Spec.Blake2s
 
-val blake2s :
-  ll:size_t{0 < size_v ll /\ size_v ll <= max_size_t - 2 * Spec.size_block } ->
-  d:lbuffer uint8 (size_v ll) -> kk:size_t{size_v kk <= 32} ->
-  k:lbuffer uint8 (size_v kk) -> nn:size_t{1 <= size_v nn /\ size_v nn <= 32} -> res:lbuffer uint8 (size_v nn) ->
+val blake2s:
+    #vll: size_nat
+  -> #vkk: size_nat
+  -> #vnn: size_nat
+  -> output: lbuffer uint8 vnn
+  -> d: lbuffer uint8 vll
+  -> ll: size_t{v ll + 2 * Spec.size_block <= max_size_t /\ v ll = vll}
+  -> kk: size_t{v kk <= 32 /\ v kk = vkk}
+  -> k: lbuffer uint8 vkk
+  -> nn:size_t{1 <= v nn /\ v nn <= 32 /\ v nn = v nn} ->
   Stack unit
-    (requires (fun h -> live h d /\ live h k /\ live h res))
-    (ensures  (fun h0 _ h1 -> preserves_live h0 h1))
+    (requires (fun h -> True))
+    (ensures  (fun h0 _ h1 -> preserves_live h0 h1 /\ modifies1 output h0 h1))
 
-let blake2s ll d kk k nn res = Hacl.Impl.Blake2s.blake2s ll d kk k nn res
+let blake2s #vll #vkk #vnn output d ll kk k nn = Hacl.Impl.Blake2s.blake2s #vll #vkk #vnn output d ll kk k nn
